binary-heap: heap-pop Qed.

binary-heap/Heap.v
@@ -2,6 +2,7 @@ Require Import Coq.Arith.Arith.
 Require Import Coq.Init.Nat.
 
 Require Import Omega.
+Require Import Coq.Logic.FunctionalExtensionality.
 
 (** Simple formalization of an array. *)
 
@@ -20,6 +21,35 @@ Definition clearv (a : array) (k : nat) : array :=
 Definition swap (a : array) (i j : nat) : array :=
   let (x, y) := (getv a i, getv a j)
   in setv (setv a i y) j x.
+
+Hint Unfold getv setv clearv swap.
+
+Lemma getv_eq :
+  forall a i v, getv (setv a i v) i = v.
+Proof.
+  intros. unfold getv. unfold setv.
+  rewrite <- beq_nat_refl. auto.
+Qed.
+
+Lemma getv_ne :
+  forall a i j v, j <> i -> getv (setv a i v) j = getv a j.
+Proof.
+  intros. unfold getv. unfold setv.
+  rewrite <- Nat.eqb_neq in H.
+  rewrite H. reflexivity.
+Qed.
+
+Lemma swap_eq :
+  forall a i, swap a i i = a.
+Proof.
+  intros.
+  apply functional_extensionality.
+  intros.
+  destruct (x =? i) eqn:H.
+  - unfold swap. unfold setv. unfold getv. rewrite H.
+    apply beq_nat_true in H. auto.
+  - unfold swap. unfold setv. unfold getv. rewrite H. auto.
+Qed.
 
 Lemma swap_get1 :
   forall a i j, getv (swap a i j) i = getv a j.
@@ -46,52 +76,7 @@ Proof.
   rewrite H. rewrite H0. reflexivity.
 Qed.
 
-(** Heap *)
-
-Definition heap : Set := array * nat.
-
-Definition heap_array (h : heap) : array :=
-  match h with
-  | (a, n) => a
-  end.
-
-Definition heap_n (h : heap) : nat :=
-  match h with
-  | (a, n) => n
-  end.
-
-Definition extend_heap (h : heap) (v : nat) : heap :=
-  (setv (heap_array h) (S (heap_n h)) v, S (heap_n h)).
-
-Definition shrink_heap (h : heap) : heap :=
-  match h with
-  | (a, 0) => (a, 0)
-  | (a, S n) => (setv a (S n) 0, n)
-  end.
-
-Definition Heap (h : heap) : Prop :=
-     (forall (i : nat), 2 <= i ->
-       getv (heap_array h) i <= getv (heap_array h) (i/2))
-  /\ (forall (i : nat), i > heap_n h -> getv (heap_array h) i = 0).
-
-Fixpoint heap_upify (h : heap) (k height : nat) : heap :=
-  match height with
-  | 0 => h
-  | S height' =>
-      if getv (heap_array h) (k/2) <? getv (heap_array h) (k)
-        then heap_upify (swap (heap_array h) k (k/2), (heap_n h)) (k/2) height'
-        else h
-  end.
-
-Definition heap_push (h : heap) (v : nat) : heap :=
-  heap_upify (extend_heap h v) (S (heap_n h)) (log2 (S (heap_n h))).
-
-Lemma extend_heap_n :
-  forall (h : heap) (v : nat),
-    heap_n (extend_heap h v) = S (heap_n h).
-Proof.
-  intros. auto.
-Qed.
+(* Some useful lemmas about log2 and division. *)
 
 Lemma log2_div2 :
   forall (k n : nat),
@@ -113,11 +98,20 @@ Proof.
   simpl. omega.
 Qed.
 
-Lemma div2_ge_k :
-  forall (n k : nat), k <= n -> k/2 <= n/2.
+Lemma div2_ge_1 :
+  forall (n : nat), 2 <= n -> 1 <= n/2.
 Proof.
   intros.
-  apply Nat.div_le_mono. omega. auto.
+  assert (2/2 <= n/2). { apply Nat.div_le_mono. omega. auto. }
+  simpl in *. auto.
+Qed.
+
+Lemma div2_ge_2 :
+  forall (n : nat), 4 <= n -> 2 <= n/2.
+Proof.
+  intros.
+  assert (4/2 <= n/2). { apply Nat.div_le_mono. omega. auto. }
+  simpl in *. auto.
 Qed.
 
 Lemma div2_le_n :
@@ -149,6 +143,39 @@ Proof.
   rewrite H in H0. omega.
 Qed.
 
+Lemma div2_mul2_vals :
+  forall (n : nat), n = 2 * (n / 2) \/ n = 2 * (n / 2) + 1.
+Proof.
+  intros. remember (n/2) as k.
+  assert (2 * k <= n). { rewrite Heqk. apply Nat.mul_div_le. omega. }
+  Check Nat.mod_eq.
+  assert (n mod 2 = n - 2 * (n/2)). { apply Nat.mod_eq. omega. }
+  rewrite <- Heqk in H0.
+  assert (n mod 2 < 2). { apply Nat.mod_upper_bound. omega. }
+  rewrite H0 in H1.
+  assert (n - 2 * k = 0 \/ n - 2 * k = 1). { omega. }
+  destruct H2.
+  - left. omega.
+  - right. omega.
+Qed.
+
+(* TODO: Prove via div2_mul2_vals. *)
+Lemma div2_neq_n :
+  forall (n k : nat), k <> 2*n -> k <> 2*n+1 -> k/2 <> n.
+Proof.
+  intros. intro contra.
+  assert (2 * n <= k). { rewrite <- contra. apply Nat.mul_div_le. omega. }
+  Check Nat.mod_eq.
+  assert (k mod 2 = k - 2 * (k/2)). { apply Nat.mod_eq. omega. }
+  rewrite contra in H2.
+  assert (k mod 2 < 2). { apply Nat.mod_upper_bound. omega. }
+  rewrite H2 in H3.
+  assert (k - 2 * n = 0 \/ k - 2 * n = 1). { omega. }
+  destruct H4.
+  - apply H. omega.
+  - apply H0. omega.
+Qed.
+
 Lemma div2_mul2_le :
   forall (n : nat), 2*(n/2) <= n.
 Proof.
@@ -156,27 +183,126 @@ Proof.
   apply Nat.mul_div_le. omega.
 Qed.
 
-Lemma div_2_2 : 1 = 2/2.
-Proof. auto. Qed.
+Lemma mul2_div2 :
+  forall (n : nat), 2*n/2 = n.
+Proof.
+  intros.
+  rewrite Nat.mul_comm, Nat.div_mul; auto.
+Qed.
 
-Lemma div_4_2 : 2 = 4/2.
-Proof. auto. Qed.
+Lemma mul2_S_div2 :
+  forall (n : nat), (2*n+1)/2 = n.
+Proof.
+  intros. symmetry.
+  eapply Nat.div_unique. auto. reflexivity.
+Qed.
 
-Hint Resolve div2_ge_k.
+Hint Resolve div2_ge_1 div2_ge_2.
 Hint Resolve div2_lt_n.
 Hint Resolve div2_le_n.
 Hint Resolve div2_eq_n.
+Hint Resolve div2_neq_n.
 Hint Resolve div2_mul2_le.
+Hint Resolve mul2_div2.
+Hint Resolve mul2_S_div2.
 Hint Resolve gt_le_S.
 Hint Resolve Nat.le_trans.
 Hint Resolve Nat.lt_le_incl.
+
+(** Heap *)
+
+Definition heap : Set := array * nat.
+
+Definition heap_array (h : heap) : array :=
+  match h with
+  | (a, n) => a
+  end.
+
+Definition heap_n (h : heap) : nat :=
+  match h with
+  | (a, n) => n
+  end.
+
+Definition extend_heap (h : heap) (v : nat) : heap :=
+  (setv (heap_array h) (S (heap_n h)) v, S (heap_n h)).
+
+Definition shrink_heap (h : heap) : heap :=
+  match h with
+  | (a, 0) => (a, 0)
+  | (a, S n) => (setv (swap a 1 (S n)) (S n) 0, n)
+  end.
+
+Definition Heap (h : heap) : Prop :=
+     (forall (i : nat), 2 <= i ->
+       getv (heap_array h) i <= getv (heap_array h) (i/2))
+  /\ (forall (i : nat), i > heap_n h -> getv (heap_array h) i = 0).
+
+Fixpoint heap_upify (h : heap) (k height : nat) : heap :=
+  match height with
+  | 0 => h
+  | S height' =>
+      if getv (heap_array h) (k/2) <? getv (heap_array h) (k)
+        then heap_upify (swap (heap_array h) k (k/2), heap_n h) (k/2) height'
+        else h
+  end.
+
+Fixpoint heap_downify (h : heap) (k height : nat) : heap :=
+  match height with
+  | 0 => h
+  | S height' =>
+      let
+        ind := if getv (heap_array h) (2*k) <? getv (heap_array h) (2*k+1)
+                 then 2*k+1
+                 else 2*k
+      in
+        if getv (heap_array h) k <? getv (heap_array h) ind
+          then heap_downify (swap (heap_array h) k ind, heap_n h) ind height'
+          else h
+  end.
+
+Definition heap_push (h : heap) (v : nat) : heap :=
+  heap_upify (extend_heap h v) (S (heap_n h)) (log2 (S (heap_n h))).
+
+Definition heap_pop (h : heap) : (heap * option nat) :=
+  match (heap_n h) with
+  | 0 => (h, None)
+  | S n => (heap_downify (shrink_heap h) 1 (log2 n), Some (heap_array h 1))
+  end.
+
+Lemma extend_heap_n :
+  forall (h : heap) (v : nat),
+    heap_n (extend_heap h v) = S (heap_n h).
+Proof.
+  intros. auto.
+Qed.
+
+Lemma shrink_heap_n :
+  forall (h : heap),
+    heap_n (shrink_heap h) = pred (heap_n h).
+Proof.
+  intros. unfold shrink_heap. unfold heap_n.
+  destruct h. destruct n; auto.
+Qed.
+
+Lemma extend_heap_unaffected :
+  forall (i v : nat) (h : heap),
+    i <> S (heap_n h) ->
+    getv (heap_array (extend_heap h v)) i = getv (heap_array h) i.
+Proof.
+  intros.
+  simpl.
+  unfold setv. unfold getv.
+  destruct (i =? S (heap_n h)) eqn:H1.
+  - apply beq_nat_true in H1. subst. omega.
+  - reflexivity.
+Qed.
 
 Lemma heap_upify_correct :
   forall (h : heap) (k height : nat),
     log2 k = height ->
     k > 0 /\ k <= heap_n h ->
     (forall (i : nat),
-       2 <= i /\ ~(k = i) -> getv (heap_array h) i <= getv (heap_array h) (i/2)) ->
+       2 <= i /\ k <> i -> getv (heap_array h) i <= getv (heap_array h) (i/2)) ->
     (forall (i : nat),
        4 <= i /\ i/2 = k -> getv (heap_array h) i <= getv (heap_array h) (k/2)) ->
     (forall (i : nat),
@@ -200,7 +326,7 @@ Proof.
     + rewrite Nat.ltb_lt in H4.
       apply IHheight; clear IHheight.
       * apply log2_div2; auto. destruct H0. auto.
-      * assert (2/2 <= k/2). { apply div2_ge_k. omega. }
+      * assert (1 <= k/2). { assert (2 <= k). { omega. } auto. }
         split; auto.
         assert (k/2 <= k). { auto. }
         destruct H0. simpl. eauto.
@@ -230,7 +356,7 @@ Proof.
         unfold heap_array.
         { destruct (k =? i) eqn:H7.
           - apply beq_nat_true in H7. subst.
-            assert (2 <= i/2). { rewrite div_4_2. apply Nat.div_le_mono; auto. rewrite <- div_4_2. auto. }
+            assert (2 <= i/2). { auto. }
             assert (i/2 < i). { apply div2_lt_n. omega. }
             assert (i/2/2 <= i/2). { apply div2_le_n. }
             assert (i/2/2 < i/2). { apply div2_lt_n. omega. }
@@ -238,14 +364,14 @@ Proof.
             rewrite swap_get3.
             apply H1. omega. omega. omega.
           - apply beq_nat_false in H7.
-            assert (2 <= i/2). { rewrite div_4_2. apply Nat.div_le_mono; auto. rewrite <- div_4_2. auto. }
+            assert (2 <= i/2). { auto. }
             assert (i/2 < i). { apply div2_lt_n. omega. }
             assert (i <> k/2). { intros contra. subst. apply div2_eq_n in H6. omega. }
-            assert (2*(k/2) <= k). { apply Nat.mul_div_le. omega. }
+            assert (2*(k/2) <= k). { auto. }
             assert (4 <= k). { rewrite <- H6 in H11. omega. }
             assert (2 <= k/2). { rewrite <- H6 in H11. omega. }
             assert (k/2 < k). { apply div2_lt_n. omega. }
-            assert (2 <= k/2). { rewrite div_4_2. apply Nat.div_le_mono; auto. rewrite <- div_4_2. auto. }
+            assert (2 <= k/2). { auto. }
             assert (k/2/2 < k/2). { apply div2_lt_n. omega. }
             rewrite swap_get3. rewrite swap_get3.
             eapply Nat.le_trans. apply H1. omega.
@@ -262,19 +388,6 @@ Proof.
         { - apply beq_nat_true in H6. subst. auto. }
         { - apply beq_nat_false in H6. auto. }
       * auto.
-Qed.
-
-Lemma extend_heap_unaffected :
-  forall (i v : nat) (h : heap),
-    i <> S (heap_n h) ->
-    getv (heap_array (extend_heap h v)) i = getv (heap_array h) i.
-Proof.
-  intros.
-  simpl.
-  unfold setv. unfold getv.
-  destruct (i =? S (heap_n h)) eqn:H1.
-  - apply beq_nat_true in H1. subst. omega.
-  - reflexivity.
 Qed.
 
 Theorem heap_push_correct :
@@ -313,4 +426,203 @@ Proof.
     assert (getv (heap_array (extend_heap h v)) i = getv (heap_array h) i).
     { apply extend_heap_unaffected. omega. }
     rewrite H2. auto.
+Qed.
+
+Lemma heap_downify_correct :
+  forall (h : heap) (k height : nat),
+    log2 k + height = log2 (heap_n h) ->
+    k > 0 ->
+    (forall (i : nat),
+       2 <= i /\ k <> i/2 -> getv (heap_array h) i <= getv (heap_array h) (i/2)) ->
+    (forall (i : nat),
+       4 <= i /\ i/2 = k -> getv (heap_array h) i <= getv (heap_array h) (k/2)) ->
+    (forall (i : nat),
+       i > heap_n h -> getv (heap_array h) i = 0) ->
+    Heap (heap_downify h k height).
+Proof.
+  intros h k height.
+  generalize dependent h.
+  generalize dependent k.
+  induction height.
+  - intros. rewrite <- plus_n_O in H.
+    assert (heap_n h < 2*k).
+    { apply Nat.log2_lt_cancel. rewrite Nat.log2_double. omega. omega. }
+    unfold Heap. split; unfold heap_downify.
+    + intros.
+      destruct (k =? (i/2)) eqn:H6.
+      * apply beq_nat_true in H6.
+        assert (heap_n h < i). { assert (2*(i/2) <= i). { auto. } omega. }
+        rewrite H3; omega.
+      * apply beq_nat_false in H6.
+        apply H1. auto.
+    + auto.
+  - intros. unfold heap_downify. fold heap_downify.
+    destruct (getv (heap_array h) (2 * k) <? getv (heap_array h) (2 * k + 1)) eqn:H4.
+    + rewrite Nat.ltb_lt in H4.
+      destruct (getv (heap_array h) k <? getv (heap_array h) (2 * k + 1)) eqn:H5.
+      * { rewrite Nat.ltb_lt in H5.
+          apply IHheight; clear IHheight.
+          - rewrite Nat.log2_succ_double. simpl. omega. auto.
+          - omega.
+          - intros. destruct H6. unfold heap_array.
+            destruct (i =? k) eqn:H8.
+            + apply beq_nat_true in H8. subst.
+              assert (k/2 < k). { auto. }
+              rewrite swap_get1. rewrite swap_get3; try omega.
+              apply H2. split. omega. auto.
+            + apply beq_nat_false in H8.
+              destruct (i =? 2*k) eqn:H9.
+              * apply beq_nat_true in H9. subst.
+                rewrite swap_get3; try omega.
+                assert (2*k/2 = k). { auto. }
+                rewrite H9. rewrite swap_get1. auto.
+              * apply beq_nat_false in H9. subst.
+                { destruct (i =? 2*k+1) eqn:H10.
+                  - apply beq_nat_true in H10. subst.
+                    rewrite swap_get2.
+                    assert ((2*k+1)/2 = k). { auto. }
+                    rewrite H10. rewrite swap_get1. auto.
+                  - apply beq_nat_false in H10.
+                    assert (i/2 <> k). { auto. }
+                    rewrite swap_get3; auto.
+                    rewrite swap_get3; auto.
+                }
+          - intros. destruct H6.
+            assert ((2*k+1)/2 = k). { auto. }
+            assert (i/2 < i). { apply div2_lt_n. omega. }
+            rewrite -> H8.
+            unfold heap_array. rewrite swap_get3. rewrite swap_get1.
+            rewrite <- H7. apply H1. omega. omega. omega.
+          - unfold heap_n, heap_array in *. intros. destruct h.
+            assert (k < n). { apply Nat.log2_lt_cancel. omega. }
+            destruct (i =? 2*k+1) eqn:H8.
+            + apply beq_nat_true in H8.
+              assert (getv a (2*k+1) = 0). { apply H3. omega. }
+              omega.
+            + apply beq_nat_false in H8. rewrite swap_get3. apply H3.
+              omega. omega. omega.
+        }
+      * { rewrite Nat.ltb_ge in H5.
+          unfold Heap. split.
+          - intros.
+            destruct (k =? i/2) eqn:H7.
+            + apply beq_nat_true in H7. subst.
+              assert (i = 2 * (i / 2) \/ i = 2 * (i / 2) + 1). { apply div2_mul2_vals. }
+              destruct H7; rewrite <- H7 in *; eauto.
+            + apply beq_nat_false in H7.
+              apply H1. auto.
+          - auto.
+        }
+    + (* almost duplicate proof as last bullet. *)
+      rewrite Nat.ltb_ge in H4.
+      destruct (getv (heap_array h) k <? getv (heap_array h) (2 * k)) eqn:H5.
+      * { rewrite Nat.ltb_lt in H5.
+          apply IHheight; clear IHheight.
+          - rewrite Nat.log2_double. simpl. omega. auto.
+          - omega.
+          - intros. destruct H6. unfold heap_array.
+            destruct (i =? k) eqn:H8.
+            + apply beq_nat_true in H8. subst.
+              assert (k/2 < k). { auto. }
+              rewrite swap_get1. rewrite swap_get3; try omega.
+              apply H2. split. omega. auto.
+            + apply beq_nat_false in H8.
+              destruct (i =? 2*k+1) eqn:H9.
+              * apply beq_nat_true in H9. subst.
+                rewrite swap_get3; try omega.
+                assert ((2*k+1)/2 = k). { auto. }
+                rewrite H9. rewrite swap_get1. auto.
+              * apply beq_nat_false in H9. subst.
+                { destruct (i =? 2*k) eqn:H10.
+                  - apply beq_nat_true in H10. subst.
+                    rewrite swap_get2.
+                    assert (2*k/2 = k). { auto. }
+                    rewrite H10. rewrite swap_get1. auto.
+                  - apply beq_nat_false in H10.
+                    assert (i/2 <> k). { auto. }
+                    rewrite swap_get3; auto.
+                    rewrite swap_get3; auto.
+                }
+          - intros. destruct H6.
+            assert (2*k/2 = k). { auto. }
+            assert (i/2 < i). { apply div2_lt_n. omega. }
+            rewrite -> H8.
+            unfold heap_array. rewrite swap_get3. rewrite swap_get1.
+            rewrite <- H7. apply H1. omega. omega. omega.
+          - unfold heap_n, heap_array in *. intros. destruct h.
+            assert (k < n). { apply Nat.log2_lt_cancel. omega. }
+            destruct (i =? 2*k) eqn:H8.
+            + apply beq_nat_true in H8.
+              assert (getv a (2*k) = 0). { apply H3. omega. }
+              omega.
+            + apply beq_nat_false in H8. rewrite swap_get3. apply H3.
+              omega. omega. omega.
+        }
+      * { rewrite Nat.ltb_ge in H5.
+          unfold Heap. split.
+          - intros.
+            destruct (k =? i / 2) eqn:H7.
+            + apply beq_nat_true in H7. subst.
+              assert (i = 2 * (i / 2) \/ i = 2 * (i / 2) + 1). { apply div2_mul2_vals. }
+              destruct H7; rewrite <- H7 in *; eauto.
+            + apply beq_nat_false in H7.
+              apply H1. auto.
+          - auto.
+        }
+Qed.
+
+Theorem heap_pop_correct :
+  forall (h : heap),
+  Heap h -> Heap (fst (heap_pop h)).
+Proof.
+  intros.
+  unfold heap_pop.
+  destruct (heap_n h) eqn:H1.
+  - auto.
+  - simpl.
+    destruct n.
+    + simpl. unfold shrink_heap.
+      destruct h. simpl in H1. subst.
+      unfold Heap in *. destruct H. unfold heap_array in *.
+      rewrite swap_eq.
+      split.
+      * intros. simpl in H0. rewrite getv_ne. rewrite H0.
+        omega. omega. omega.
+      * intros. simpl in H0.
+        destruct (i =? 1) eqn:H2.
+        apply beq_nat_true in H2. subst. auto.
+        apply beq_nat_false in H2. rewrite getv_ne. rewrite H0.
+        auto. omega. omega.
+    + apply heap_downify_correct; try omega.
+      * rewrite Nat.log2_1. rewrite shrink_heap_n. rewrite H1.
+        auto.
+      * intros. destruct H0. unfold Heap in H. destruct H.
+        unfold shrink_heap. unfold heap_array in *. destruct h.
+        unfold heap_n in *. subst.
+        destruct (i/2 =? S (S n)) eqn:H4.
+        { - apply beq_nat_true in H4. rewrite -> H4.
+            assert (S (S n) < i). { assert (i / 2 < i). { auto. } omega. }
+            rewrite getv_ne. rewrite getv_eq.
+            rewrite swap_get3. rewrite H3.
+            omega. omega. omega. omega. omega.
+        }
+        { - apply beq_nat_false in H4.
+            destruct (i =? S (S n)) eqn:H5.
+            + apply beq_nat_true in H5. subst.
+              rewrite getv_eq. omega.
+            + apply beq_nat_false in H5.
+              rewrite getv_ne. rewrite getv_ne.
+              rewrite swap_get3. rewrite swap_get3. apply H.
+              omega. omega. omega. omega. omega. omega. omega.
+        }
+      * intros. destruct H0.
+        assert (2 <= i/2). { auto. } omega.
+      * intros. rewrite shrink_heap_n in H0. rewrite H1 in H0. simpl in H0.
+        unfold Heap in H. destruct H. rewrite H1 in H2.
+        unfold shrink_heap, heap_array. destruct h. unfold heap_n in H1.
+        subst.
+        destruct (i =? S (S n)) eqn:H3.
+        { apply beq_nat_true in H3. subst. rewrite getv_eq. auto. }
+        { apply beq_nat_false in H3. rewrite getv_ne, swap_get3.
+          apply H2. omega. omega. omega. omega. }
 Qed.
